src/cbor/pulse/raw/CBOR.Pulse.Raw.Match.fst
@@ -1114,7 +1114,6 @@ fn cbor_string_reset_perm_correct
     fold (cbor_match_string c p r)
   };
   rewrite each c' as cbor_string_reset_perm (p /. q) c;
-  ()
 }
 
 ghost
@@ -1138,8 +1137,10 @@ fn cbor_tagged_reset_perm_correct
   with s . assert (pts_to c.cbor_tagged_ptr #(p `perm_mul` c.cbor_tagged_ref_perm) s);
   rewrite (pts_to c.cbor_tagged_ptr #(p `perm_mul` c.cbor_tagged_ref_perm) s)
     as (pts_to c'.cbor_tagged_ptr #(q `perm_mul` c'.cbor_tagged_ref_perm) s);
-  with c_ . rewrite cbor_match (perm_mul p c.cbor_tagged_payload_perm) c_ (Tagged?.v r)
-    as cbor_match (perm_mul q c'.cbor_tagged_payload_perm) c_ (Tagged?.v r);
+  with c_ . rewrite
+    cbor_match (perm_mul p c.cbor_tagged_payload_perm) c_ (Tagged?.v r)
+  as
+    cbor_match (perm_mul q c'.cbor_tagged_payload_perm) c_ (Tagged?.v r);
   fold (cbor_match_tagged c' q r cbor_match);
   intro
     (Trade.trade
@@ -1266,7 +1267,7 @@ fn cbor_raw_reset_perm_correct
         Trade.rewrite_with_trade
           (cbor_match_string (cbor_string_reset_perm (p /. q) v) q r)
           (cbor_match q c' r);
-        rewrite each c' as cbor_raw_reset_perm_tot (p /. q) c;
+        rewrite each c' as (cbor_raw_reset_perm_tot (p /. q) c);
         Trade.trans _ _ (cbor_match p c r)
     }
     norewrite
@@ -1276,8 +1277,7 @@ fn cbor_raw_reset_perm_correct
         (cbor_match_int v r);
       Trade.rewrite_with_trade
         (cbor_match_int v r)
-        (cbor_match q c r);
-      rewrite each (cbor_match q c r) as (cbor_match q (cbor_raw_reset_perm_tot (p /. q) c) r);
+        (cbor_match q (cbor_raw_reset_perm_tot (p /. q) c) r);
       Trade.trans _ _ (cbor_match p c r)
     }
     norewrite
@@ -1287,8 +1287,7 @@ fn cbor_raw_reset_perm_correct
         (cbor_match_simple v r);
       Trade.rewrite_with_trade
         (cbor_match_simple v r)
-        (cbor_match q c r);
-      rewrite each (cbor_match q c r) as (cbor_match q (cbor_raw_reset_perm_tot (p /. q) c) r);
+        (cbor_match q (cbor_raw_reset_perm_tot (p /. q) c) r);
       Trade.trans _ _ (cbor_match p c r)
     }
     norewrite
@@ -1303,7 +1302,7 @@ fn cbor_raw_reset_perm_correct
       Trade.rewrite_with_trade
         (cbor_match_tagged (cbor_tagged_reset_perm (p /. q) v) q r cbor_match)
         (cbor_match q c' r);
-      rewrite each c' as cbor_raw_reset_perm_tot (p /. q) c;
+      rewrite each c' as (cbor_raw_reset_perm_tot (p /. q) c);
       Trade.trans _ _ (cbor_match p c r)
     }
     norewrite
@@ -1318,7 +1317,7 @@ fn cbor_raw_reset_perm_correct
       Trade.rewrite_with_trade
         (cbor_match_array (cbor_array_reset_perm (p /. q) v) q r cbor_match)
         (cbor_match q c' r);
-      rewrite each c' as cbor_raw_reset_perm_tot (p /. q) c;
+      rewrite each c' as (cbor_raw_reset_perm_tot (p /. q) c);
       Trade.trans _ _ (cbor_match p c r)
     }
     norewrite
@@ -1333,7 +1332,7 @@ fn cbor_raw_reset_perm_correct
       Trade.rewrite_with_trade
         (cbor_match_map0 (cbor_map_reset_perm (p /. q) v) q r cbor_match)
         (cbor_match q c' r);
-      rewrite each c' as cbor_raw_reset_perm_tot (p /. q) c;
+      rewrite each c' as (cbor_raw_reset_perm_tot (p /. q) c);
       Trade.trans _ _ (cbor_match p c r)
     }
     norewrite
@@ -1341,24 +1340,21 @@ fn cbor_raw_reset_perm_correct
       perm_q_p_r q p s.cbor_serialized_perm;
       Trade.rewrite_with_trade
         (cbor_match p c r)
-        (cbor_match q c' r);
-      rewrite each c' as cbor_raw_reset_perm_tot (p /. q) c;
+        (cbor_match q (cbor_raw_reset_perm_tot (p /. q) c) r)
     }
     norewrite
     CBOR_Case_Serialized_Array s -> {
       perm_q_p_r q p s.cbor_serialized_perm;
       Trade.rewrite_with_trade
         (cbor_match p c r)
-        (cbor_match q c' r);
-      rewrite each c' as cbor_raw_reset_perm_tot (p /. q) c;
+        (cbor_match q (cbor_raw_reset_perm_tot (p /. q) c) r)
     }
     norewrite
     CBOR_Case_Serialized_Map s -> {
       perm_q_p_r q p s.cbor_serialized_perm;
       Trade.rewrite_with_trade
         (cbor_match p c r)
-        (cbor_match q c' r);
-      rewrite each c' as cbor_raw_reset_perm_tot (p /. q) c;
+        (cbor_match q (cbor_raw_reset_perm_tot (p /. q) c) r)
     }
   }
 }
