src/cbor/spec/raw/everparse/CBOR.Spec.Raw.Format.fst
@@ -199,8 +199,6 @@ let serialize_array_eq
   LP.serialize_dtuple2_eq F.serialize_header F.serialize_content v1';
   LowParse.Spec.VCList.tot_serialize_nlist_serialize_nlist (List.Tot.length x1) F.tot_serialize_raw_data_item x1
 
-#pop-options
-
 let serialize_cbor_array_length_gt_list len l =
   serialize_array_eq len l;
   LP.serialize_length F.serialize_header (F.raw_uint64_as_argument cbor_major_type_array len)
@@ -227,8 +225,6 @@ let serialize_string_eq
   let v1' = F.synth_raw_data_item_recip v1 in
   LP.serialize_dtuple2_eq F.serialize_header F.serialize_content v1';
   ()
-
-#push-options "--z3rlimit 32"
 
 let serialize_cbor_string_length_gt ty len l =
   serialize_string_eq ty len l;
@@ -369,7 +365,7 @@ let parse_cbor_map_prefix
       s1 s2
   | _ -> ()
 
-#push-options "--z3rlimit_factor 4"
+#push-options "--z3rlimit_factor 8"
 
 let parse_cbor_map_equiv
   (n: nat)
