src/lowparse/pulse/LowParse.Pulse.Recursive.fst
@@ -124,10 +124,6 @@ let validate_tot_nlist_recursive_overflow
   let offset = off + consumed in
   parse_nlist_recursive_bound_correct p (p.count h + (n - 1)) (Seq.slice v (offset) (Seq.length v))
 
-#pop-options
-
-#restart-solver
-
 inline_for_extraction
 fn validate_tot_nlist_recursive
   (#p: Ghost.erased parse_recursive_param)
@@ -208,6 +204,8 @@ fn validate_tot_nlist_recursive
 }
 
 #pop-options
+
+#restart-solver
 
 inline_for_extraction
 fn validate_nlist_recursive
